p4cub has type variables...

deps/poulet4/lib/P4cub/BigStep/Value/Auxilary.v
@@ -3,19 +3,25 @@ Require Import Poulet4.P4cub.BigStep.Value.Syntax
 Import Val ValueNotations P.P4cubNotations.
 
 (** Intial/Default value from a type. *)
-Fixpoint vdefault (τ : E.t) : v :=
+Fixpoint vdefault (τ : E.t) : option v :=
   match τ with
-  | {{ error }}      => ~{ ERROR None }~
-  | {{ matchkind }}  => ~{ MATCHKIND exact }~
-  | {{ Bool }}       => ~{ FALSE }~
-  | {{ bit<w> }}     => VBit w 0%Z
-  | {{ int<w> }}     => VInt w 0%Z
-  | {{ tuple ts }}   => VTuple $ List.map vdefault ts
-  | {{ struct { ts } }} => VStruct $ F.map vdefault ts
-  | {{ hdr { ts } }} => VHeader (F.map vdefault ts) false
-  | {{ stack fs[n] }} => VHeaderStack
-                          fs (repeat (false, F.map vdefault fs)
-                                     (Pos.to_nat n)) n 0
+  | {{ error }}      => Some ~{ ERROR None }~
+  | {{ matchkind }}  => Some ~{ MATCHKIND exact }~
+  | {{ Bool }}       => Some ~{ FALSE }~
+  | {{ bit<w> }}     => Some $ VBit w 0%Z
+  | {{ int<w> }}     => Some $ VInt w 0%Z
+  | {{ tuple ts }}
+    => vs <<| sequence $ List.map vdefault ts ;; VTuple vs
+  | {{ struct { ts } }}
+    => vs <<| sequence $ List.map (fun '(x,t) => v <<| vdefault t ;; (x, v)) ts ;;
+      ~{ STRUCT { vs } }~
+  | {{ hdr { ts } }}
+    => vs <<| sequence $ List.map (fun '(x,t) => v <<| vdefault t ;; (x, v)) ts ;;
+      ~{ HDR { vs } VALID:=false }~
+  | {{ stack ts[n] }}
+    => vs <<| sequence $ List.map (fun '(x,t) => v <<| vdefault t ;; (x, v)) ts ;;
+      VHeaderStack ts (repeat (false, vs) (Pos.to_nat n)) n 0
+  | E.TVar _ => None
   end.
 (**[]*)
 
