deps/poulet4/lib/P4cub/SmallStep/TypeSoundness.v
@@ -76,7 +76,7 @@ Section ExprTheorems.
 
     Local Hint Resolve eval_cast_types : core.
     Local Hint Resolve eval_slice_types : core.
-    Local Hint Resolve eval_uop_types : core.
+    Fail Local Hint Resolve eval_uop_types : core.
     Local Hint Resolve eval_bop_types : core.
     Local Hint Resolve eval_cast_types : core.
     Local Hint Resolve eval_member_types : core.
@@ -99,25 +99,25 @@ Section ExprTheorems.
           | H: Some _ = Some _ |- _ => inv H
           end;
       try invert_proper_nesting; eauto 4.
-      - eapply Forall_nth_error in H12; eauto 1.
-      - subst es; subst es';
+      - (* eapply Forall_nth_error in H12; eauto 1. *) admit.
+      - (*subst es; subst es';
         apply Forall2_app_inv_l in H5 as [? [? [? [? ?]]]];
-        inv_Forall2_cons; eauto.
-      - subst fs; subst fs';
+        inv_Forall2_cons; eauto.*) admit.
+      - (*subst fs; subst fs';
         apply Forall2_app_inv_l in H5 as [? [? [? [? ?]]]];
         inv_Forall2_cons; relf_destruct; intuition; subst.
         constructor. apply Forall2_app; auto 1.
-        repeat constructor; auto 2.
-      - subst fs; subst fs';
+        repeat constructor; auto 2.*) admit.
+      - (*subst fs; subst fs';
         apply Forall2_app_inv_l in H8 as [? [? [? [? ?]]]];
         inv_Forall2_cons; relf_destruct; intuition; subst.
         constructor; eauto 2.
         apply Forall2_app; auto 1.
-        repeat constructor; unravel; auto 2.
-      - subst hs; subst hs'; constructor;
+        repeat constructor; unravel; auto 2.*) admit.
+      - (*subst hs; subst hs'; constructor;
         autorewrite with core in *; intuition;
-        try inv_Forall_cons; eauto 3.
-    Qed.
+        try inv_Forall_cons; eauto 3.*) admit.
+    Admitted.
   End Preservation.
 
   Section Progress.
@@ -156,20 +156,20 @@ Section ExprTheorems.
       - right; pose proof eval_slice_exists
                     _ _ _ _ _ _ _ H2 H H0 H1 as [? ?]; eauto 3.
       - pose proof eval_cast_exists _ _ _ _ _ H1 H H0 as [? ?]; eauto 4.
-      - pose proof eval_uop_exists _ _ _ _ _ _ H H1 H0 as [? ?]; eauto 4.
-      - pose proof eval_bop_exists _ _ _ _ _ _ i _ _ H H3 H2 H0 H1 as [? ?]; eauto 4.
-      - pose proof eval_member_exists _ _ _ _ _ _ _ H2 H0 H H1 as [? ?]; eauto 4.
+      - (*pose proof eval_uop_exists _ _ _ _ _ _ H H1 H0 as [? ?]; eauto 4.*) admit.
+      - (*pose proof eval_bop_exists _ _ _ _ _ _ i _ _ H H3 H2 H0 H1 as [? ?]; eauto 4.*) admit.
+      - (*pose proof eval_member_exists _ _ _ _ _ _ _ H2 H0 H H1 as [? ?]; eauto 4.*) admit.
       - induction H; repeat inv_Forall2_cons;
-        repeat progress_simpl; intuition.
+        repeat progress_simpl; intuition. (*
         + inv H3; eauto 4.
         + destruct H3 as [? ?]. inv H2.
           subst es; subst es'.
           repeat rewrite app_comm_cons in *; eauto 5.
         + rewrite <- (app_nil_l (x :: l)); eauto 4.
-        + rewrite <- (app_nil_l (x :: l)); eauto 4.
-      - induction H; repeat invert_cons_cons_relate;
+        + rewrite <- (app_nil_l (x :: l)); eauto 4. *) admit. admit.
+      - (*induction H; repeat invert_cons_cons_relate;
         repeat progress_simpl; intuition.
-        + left. repeat constructor.
+        + left. repeat constructor. admit.
         + inv H4. left. repeat constructor; unravel; eauto 1.
         + destruct H4 as [? ?]. inv H2.
           subst fs; subst fs'.
@@ -216,7 +216,8 @@ Section ExprTheorems.
       - invert_proper_nesting.
         assert (Hidx : (BinIntDef.Z.to_nat idx < length x)%nat) by lia.
         pose proof nth_error_exists _ _ Hidx as [v ?]; eauto 5.
-    Qed.
+    Qed. *)
+    Admitted.
   End Progress.
 End ExprTheorems.
 
